src/facts.v
@@ -38,52 +38,83 @@ Defined.
 Theorem king_cant_move_into_attack : forall game_state (from to : Square),
     get_square game_state.(board) from = Some {| piece:=King; color:= game_state.(player_turn) |} ->
     SquareSet.In to (valid_moves game_state from) ->
-    is_attacked (game_state.(board)) to (game_state.(player_turn)) = false.
+    is_attacked game_state.(board) game_state.(player_turn) to = false.
 Proof.
   intros.
   unfold valid_moves in H0. simpl in H0. rewrite H in H0. rewrite color_eq_refl in H0. 
-  destruct (is_in_check game_state); apply SquareSet.filter_2 in H0;
+  destruct (is_in_check game_state.(board) game_state.(player_turn)); apply SquareSet.filter_2 in H0;
     try (apply andb_prop in H0; destruct H0; apply negb_true_iff in H0; apply H0);
     unfold compat_bool; unfold Proper; unfold "==>"; intros; rewrite square_eq_refl in H1; destruct H1; reflexivity.
-Qed.
+Defined.
 
-Theorem get_king_correct : forall board turn square,
-    get_king board turn = Some square ->
-    get_square board square = Some {| piece := King; color := turn |}.
+Theorem get_king_correct : forall game_state square,
+    get_king game_state.(board) game_state.(player_turn) = Some square ->
+    get_square game_state.(board) square = Some {| piece := King; color := game_state.(player_turn) |}.
 Proof.
   intros.
-  unfold get_king in H. unfold get_square. 
+  unfold get_king in H. unfold get_square.
   destruct (OrdSquareMapProp.min_elt
               (moves.SquareMapProp.filter
                  (fun (_ : SquareMap.key) (p : ColoredPiece) =>
-                    is_king (piece p) && color_equal turn (color p)) board)) eqn:E; try discriminate.
+                    is_king (piece p) &&
+                      color_equal (player_turn game_state) (color p)) (board game_state))) eqn:E; try discriminate.
   destruct p. simpl in H. inversion H; subst; clear H.
   apply OrdSquareMapProp.min_elt_MapsTo in E.
   apply SquareMapProp.filter_iff in E.
   - destruct E. apply SquareMap.find_1 in H. destruct c.
-    apply andb_prop in H0 as [King Color]. destruct piece; destruct color; destruct turn; try discriminate; apply H.
+    apply andb_prop in H0 as [King Color]. destruct piece; destruct color; destruct game_state.(player_turn); try discriminate; apply H.
   - unfold Proper. intros sq1 sq2 G x y J. destruct J. reflexivity.
 Defined.
 
-
 Theorem needs_king_to_be_in_check : forall game_state,
-    is_in_check game_state = true ->
+    is_in_check game_state.(board) game_state.(player_turn) = true ->
     exists sq, get_square game_state.(board) sq = Some {| piece:=King; color:= game_state.(player_turn) |}.
 Proof.
-  intros. unfold is_in_check in H. destruct (get_king (board game_state) (player_turn game_state)) as [sq|] eqn:King; try discriminate.
+  intros. unfold is_in_check in H. destruct (get_king game_state.(board) game_state.(player_turn)) as [sq|] eqn:King; try discriminate.
   exists sq. apply get_king_correct in King. apply King.
 Defined.
 
 Theorem if_in_check_then_can_only_move_king : forall game_state from to,
-    is_in_check game_state = true ->
+    is_in_check game_state.(board) game_state.(player_turn) = true ->
     SquareSet.In to (valid_moves game_state from) ->
     get_square game_state.(board) from = Some {| piece:= King; color:= game_state.(player_turn)|}.
 Proof.
   intros.
   unfold valid_moves in H0. rewrite H in H0. unfold is_in_check in H.
-  destruct (get_king (board game_state) (player_turn game_state)) in H; try discriminate.
+  destruct (get_king game_state.(board) game_state.(player_turn)) in H; try discriminate.
   destruct (get_square (board game_state) from).
   - destruct c. destruct (color_equal color (player_turn game_state)) eqn:C; destruct piece eqn:P; try (apply set_is_empty in H0; destruct H0). simpl in H0. destruct color; destruct (player_turn game_state); try discriminate; reflexivity.
   - apply set_is_empty in H0. destruct H0.
 Qed.
+
+Theorem is_attacked_correct : forall game_state sq,
+    IsAttacked game_state sq <-> is_attacked game_state.(board) game_state.(player_turn) sq = true.
+Proof.
+  split; intros.
+  - unfold IsAttacked in H. unfold is_attacked. destruct H as [attacker_sq [in_attacks has_enemy_in_sq]].
+    unfold has_enemy in has_enemy_in_sq. unfold has_ally in has_enemy_in_sq.
+    rewrite SquareMapProp.exists_iff.
+    + destruct (get_square (board game_state) attacker_sq) eqn:E; try discriminate.
+      exists (attacker_sq, c). split.
+      * simpl. unfold get_square in E. apply SquareMap.find_2 in E. apply E.
+      * apply andb_true_intro. split.
+        { simpl. apply SquareSet.mem_1 in in_attacks. apply in_attacks. }
+        { destruct c. simpl. destruct color; destruct game_state.(player_turn); try discriminate; apply has_enemy_in_sq. }
+    + unfold Proper. intros sq1 sq2 G x y J. destruct J. apply square_eq_refl in G. destruct G. reflexivity.
+  - unfold IsAttacked. unfold is_attacked in H. rewrite SquareMapProp.exists_iff in H. destruct H as [[attacker_sq c_piece] [Maps Eq]].
+    exists attacker_sq. split; apply andb_prop in Eq as [Attacks ColorEq].
+    + apply SquareSet.mem_2 in Attacks. apply Attacks.
+    + unfold has_enemy. unfold has_ally. unfold get_square. apply SquareMap.find_1 in Maps. simpl in Maps. rewrite Maps.
+      destruct c_piece as [piece color]. simpl in ColorEq. destruct color; destruct game_state.(player_turn); try discriminate; apply ColorEq.
+    + unfold Proper. intros sq1 sq2 G x y J. destruct J. apply square_eq_refl in G. destruct G. reflexivity.
+Defined.
+
+Theorem is_in_check_correct : forall game_state square,
+    get_king game_state.(board) game_state.(player_turn) = Some square ->
+    is_in_check game_state.(board) game_state.(player_turn) = true <-> is_attacked game_state.(board) game_state.(player_turn) square = true.
+Proof.
+  split; intros.
+  - unfold is_in_check in H0. rewrite H in H0. apply H0.
+  - unfold is_in_check. rewrite H. apply H0.
+Defined.
 
