src/pgn.v
@@ -1,0 +1,197 @@
+Require Import board.
+Require Import moves.
+From Coq Require Import Strings.String.
+From Coq Require Import Strings.Ascii.
+From Coq Require Import Arith.Arith.
+From Coq Require Import Init.Nat.
+From Coq Require Import Arith.EqNat.
+From Coq Require Import Lists.List. Import ListNotations.
+Require Import Program.
+Require Import Lia.
+
+Inductive ParserError :=
+| InvalidPiece
+| InvalidFile 
+| InvalidRank
+| UnexpectedEOF
+| Expected (c: ascii) (got: ascii).
+
+Inductive Result {T} : Type :=
+| Ok (x: T) : @Result T
+| Err (err: ParserError) : @Result T
+.
+
+Arguments Ok {T}.
+Arguments Err {T}.
+
+Definition parser {T: Type} := list nat -> @Result (T * list nat).
+
+Fixpoint to_list s : list nat :=
+  match s with
+  | EmptyString => []
+  | String c s => (nat_of_ascii c) :: (to_list s)
+  end.
+
+Definition map {A B} (f: A -> B) (p: @parser A) : @parser B :=
+  fun s =>
+    match p s with
+    | Ok (x, rest) => Ok (f x, rest)
+    | Err err => Err err
+    end.
+
+Definition bind {A B} (r: @Result A) (f: A -> @Result B) :=
+  match r with
+  | Ok p => f p
+  | Err err => Err err
+  end.
+
+Notation "'let*' p ':=' c1 'in' c2" := (bind c1 (fun p => c2))
+    (at level 61, p as pattern, c1 at next level, right associativity).
+
+Definition parse_piece : @parser Piece :=
+  fun s =>
+    match s with
+    | 81 :: l => Ok (Queen , l)
+    | 82 :: l => Ok (Rook  , l)
+    | 75 :: l => Ok (King  , l)
+    | 80 :: l => Ok (Pawn  , l)
+    | 78 :: l => Ok (Horse , l)
+    | 66 :: l => Ok (Bishop, l)
+    | _ => Err InvalidPiece
+    end.
+
+Definition parse_file : @parser File :=
+  fun s =>
+    match s with
+    | 61 :: l | 97 :: l  => Ok (A, l)
+    | 62 :: l | 98 :: l  => Ok (B, l)
+    | 63 :: l | 99 :: l  => Ok (C, l)
+    | 64 :: l | 100 :: l => Ok (D, l)
+    | 65 :: l | 101 :: l => Ok (E, l)
+    | 66 :: l | 102 :: l => Ok (F, l)
+    | 67 :: l | 103 :: l => Ok (G, l)
+    | 68 :: l | 104 :: l => Ok (H, l)
+    | _ => Err InvalidFile
+    end.
+
+Definition parse_rank : @parser Rank :=
+  fun s =>
+    match s with
+    | 49 :: l => Ok (R1, l)
+    | 50 :: l => Ok (R2, l)
+    | 51 :: l => Ok (R3, l)
+    | 52 :: l => Ok (R4, l)
+    | 53 :: l => Ok (R5, l)
+    | 54 :: l => Ok (R6, l)
+    | 55 :: l => Ok (R7, l)
+    | 56 :: l => Ok (R8, l)
+    | _ => Err InvalidRank
+    end.
+
+Definition parse_square : @parser Square :=
+  fun s =>
+    let* (file, s) := parse_file s in
+    let* (rank, s) := parse_rank s in
+    Ok ({| file:= file; rank:= rank|}, s).
+
+Definition whitespace : @parser unit :=
+  fix ws s :=
+    match s with
+    | 32 :: l | 10 :: l => let* (_, rest) := ws l in Ok (tt, rest)
+    | _ => Ok (tt, s)
+    end.
+
+Fixpoint writeNatAux (time n : nat) (acc : string) : string :=
+  let acc' := String (ascii_of_nat (48 + (n mod 10))) acc in
+  match time with
+    | 0 => acc'
+    | S time' =>
+      match n / 10 with
+        | 0 => acc'
+        | n' => writeNatAux time' n' acc'
+      end
+  end.
+
+Definition writeNat (n : nat) : string :=
+  writeNatAux n n "".
+
+
+Definition maybe {A} (p: @parser A) : @parser (option A) :=
+  fun s =>
+    match p s with
+    | Ok (p, rest) => Ok (Some p, rest)
+    | Err err => Ok (None, s)
+    end.
+
+Definition or {A} (p1 p2: @parser A) : @parser A :=
+  fun s =>
+    match p1 s with
+    | Ok r => Ok r
+    | Err _ => p2 s
+    end.
+
+Definition expect_char (a: ascii) : @parser unit :=
+  fun s =>
+    match s with
+    | c :: rest => if Nat.eqb (nat_of_ascii a) c then
+                   Ok (tt, rest)
+                 else
+                   Err (Expected a (ascii_of_nat c))
+    | [] => Err UnexpectedEOF
+    end.
+
+Fixpoint expect_string (str: string) (rest: list nat) :=
+  match str, rest with
+  | String a s, n :: l =>
+      if Nat.eqb (nat_of_ascii a) n then
+        expect_string s l
+      else
+        Err (Expected a (ascii_of_nat n))
+  | _, [] => Err UnexpectedEOF
+  | EmptyString, _ => Ok (tt, rest)
+  end.
+
+Record SAN := {
+    from_file : option File;
+    from_rank : option Rank;
+    to : Square;
+    piece : Piece;
+    captures : bool;
+    check : bool;
+  }.
+
+Definition is_some {A} (o: option A) := match o with Some _ => true | None => false end.
+Definition or_default {A} (a: A) (o: option A) : A := match o with Some x => x | None => a end.
+
+Definition parse_san : @parser SAN :=
+  fun s =>
+    let* (p, rest) := (map (or_default Pawn) (maybe parse_piece)) s in
+    let* (maybe_f, rest) := maybe parse_file rest in
+    let* (maybe_r, rest) := maybe parse_rank rest in
+    let* (captures, rest) := maybe (expect_char "x") rest in
+    let* (sq, rest) := maybe parse_square rest in
+    let* (check, rest) := maybe (expect_char "+") rest in
+    let* (f, r, sq) :=
+      match maybe_f, maybe_r, sq with
+      | Some f, Some r, None => Ok (None, None, Build_Square f r)
+      | _, _, Some sq => Ok (maybe_f, maybe_r, sq)
+      | _, _, None => Err UnexpectedEOF
+      end in
+    Ok ({| piece := p; captures := is_some captures; from_file:=f; from_rank:=r; to:=sq; check:= is_some check |}, rest).
+
+Fixpoint parse_game (game_state: GameState) (gas: nat) (s: list nat) : @Result (ValidGame game_state) :=
+  match gas with
+  | S g =>
+      let* (_, rest)      := expect_string (writeNat turn) s in
+      let* (_, rest)      := expect_char "." rest in
+      let* (_, rest)      := whitespace rest in
+      let* (w_move, rest) := parse_san rest in
+      let* (_, rest)      := whitespace rest in
+      let* (b_move, rest) := parse_san rest in
+      let* (_, rest)      := whitespace rest in
+      let* (games, rest)  := parse_game (turn + 1) g rest in
+      Ok ((w_move, b_move)::games, rest)
+  | 0 => Ok ([], s)
+  end.
+
+Compute (parse_game 1 4 (to_list "1. e4 e5 2. Nf3 Nc6 3. Bb5 a6 4. Ba4 Nf6")).
